reduction_semantics/reduction_semantics.v
@@ -3,60 +3,9 @@ Require Import Relations
 Require Export rewriting_system.
 
 
-(* Note: The only grammar mentioned in this formalization is a grammar of evaluation
-   contexts, thus any reference to a grammar means the grammar of contexts of 
-   the formalized language.
-   
-   In this formalisation we represent evaluation contexts in terms of elementary
-   contexts (if you do not understand this go to the paper). To obtain the grammar 
-   proper for this formalization first translate the original grammar to a form, 
-   where each right side of a production is a hole or it has a context non-terminal.
-   Now if you take each non-hole right side and replace the context symbol by a hole,
-   you will a set of get context patterns that identify needed elementary contexts - 
-   we will use EC markings for these patterns.
-
-   E.g., if k1, k2 are context non-terminals and there is a production  k1 -> a b k2 c,
-   then the coresponding context pattern is  a b [] c  .
-
-   Unfortunatly, not all such grammars are proper for our formalisation, so we may 
-   still need to refine them. If we try to say it intuitivly, the grammars describe 
-   automata on words build from elementary contexts and these automata need to be 
-   deterministic.
-
-   Saying it less intuitvaly: for any context non-teminal symbol k and elem. context ec 
-   there needs to be at most one k' such that there exists a production  k -> EC[k']  
-   and ec matches EC. Let us call such grammars >deterministic grammars of contexts<. 
-
-   You may achive this form by spliting the context patterns and determinizing 
-   the grammar.
-
-   E.g., suppose you have a grammar with two productions form k1:  k1 -> a k2 a,  
-   k1 -> ab k3 ab,  where L(a), L(b) are disjoint languages and L(ab) = L(a) U L(b). 
-   Then you may split the second pattern  ab [] ab  to:  a [] a,  b [] ab,  ab [] b. 
-   So, the second production may be replaced by three other:  k1 -> a k3 a,  
-   k -> b k3 ab,  k -> ab k3 b. And then you may determinize the grammar by the
-   exponential construction. In this case, it will introduce a new context symbol 
-   {k2,k3}, replacing the productions  k1 -> a k2 a,  k1 -> a k3 a  with  
-   k1 -> a {k2,k3} a  and derivating the missing part of the grammar from the symbol
-   {k2,k3}.
-
-   In this formalisation contexts are treated as words of elementary contexts, where
-   the end of a word means a hole. Because such a word may end in any place, this 
-   enforces an additional condition on the grammars that, the production  k -> []  
-   exists for any non-terminal k. However, this condition is not restrictive (keep
-   reading).
-
-   Definition: If a derivation of a context ends with a production  k -> [], then
-   we say that the context has a >hole of the kind k<. 
-
-   In this formalisation we may give a different set of redexes that may occure in 
-   a hole per each hole kind. Hence, if there was no production  k -> [], then
-   we may equivalently fix an empty set of redexes for this k. *)
 
 
-
-
-(* Signature for languages with reduction semantics and multiple kinds of contextes. *)
+(* Signature for languages with reduction semantics. *)
 
 Module Type RED_SEM.
 
@@ -80,13 +29,6 @@ Module Type RED_SEM.
   Coercion  redex_to_term : redex >-> term.
 
 
-  (* context k1 k2 - contexts of kind k1 (derivated from k1) with a hole of kind k2. 
-                     Contexts are represented by reversed derivations in the grammar.
-                     E.g., if a context is derivated by a sequence of productions
-                     k1 -> ec1 k2, k2 -> ec2 k3, k3 -> ec3 k4, k4 -> [], then it is 
-                     represented by the list  (ec3, k3), (ec2, k2), (ec1, k1)  of 
-                     the type  context k1 k4.
-                     The second elements in the pairs are implicite. *)
   Inductive context (k1 : ckind) : ckind -> Set :=
   | empty : context k1 k1
   | ccons : forall (ec : elem_context) {k2}, context k1 k2 -> context k1 (k2+>ec).
@@ -94,12 +36,6 @@ Module Type RED_SEM.
   Notation "[.]"      := empty.
   Notation "[.]( k )" := (@empty k).
   Infix    "=:"       := ccons (at level 60, right associativity).
-
-  (* Definition: The hole of a context is called >dead< if its kind is a sink symbol. *)
-
-  (* Definition: A context is called >proper< if its hole is not dead. 
-     (Context with dead holes are contexts that cannot be generated in the orginal
-     grammar.) *)
 
   Fixpoint compose {k1 k2} (c0 : context k1 k2) 
                       {k3} (c1 : context k3 k1) : context k3 k2 := 
@@ -118,9 +54,6 @@ Module Type RED_SEM.
 
   Definition immediate_ec ec t := exists t', ec:[t'] = t.
 
-  (* decomp k - decomposition of a term t from the symbol k to a redex.
-     d_red r c  means: t = c[r].
-     d_val v    means: t has no redexes and so it is a value, t = v. *)
   Inductive decomp k : Set :=
   | d_red : forall {k'}, redex k' -> context k k' -> decomp k
   | d_val : value k -> decomp k.
@@ -146,9 +79,6 @@ Module Type RED_SEM.
   Instance rws : REWRITING_SYSTEM term :=
   { transition := reduce init_ckind }.
 
-  (* Definition: A decomposition c[t] is empty if c is empty. *)
-  (* Definition: A decomposition c[t] is proper if c is proper. *)
-
 
 
   Axioms
@@ -167,8 +97,6 @@ Module Type RED_SEM.
   (redex_to_term_injective :                                 forall {k} (r r' : redex k),
        redex_to_term r = redex_to_term r' -> r = r')
 
-  (* The following axiom, somehow, relates our representation of contexts to the real
-     reduction contexts. *)
   (elem_plug_injective1 :                                                forall ec t0 t1,
        ec:[t0] = ec:[t1] -> t0 = t1)
 
