refocusing/refocusing_semantics_facts.v
@@ -12,8 +12,8 @@ Module RED_REF_SEM_Facts (R : RED_REF_SEM).
   Import R RF.
 
 
-  Lemma dec_proc_starts_alive :                   forall t {k1 k2} (c : context k1 k2) d,
-      dec_proc t c d -> ~dead_ckind k2.
+  Lemma refocus_in_starts_alive :                 forall t {k1 k2} (c : context k1 k2) d,
+      refocus_in t c d -> ~dead_ckind k2.
 
   Proof.
     intros t k1 k2 c d H H0.
@@ -27,8 +27,9 @@ Module RED_REF_SEM_Facts (R : RED_REF_SEM).
   Qed.
 
 
-  Lemma decctx_proc_starts_alive : forall {k2} (v : value k2) {k1} (c : context k1 k2) d,
-      decctx_proc v c d -> ~dead_ckind k2.
+  Lemma refocus_out_starts_alive :                        forall {k2} (v : value k2) {k1}
+                                                                   (c : context k1 k2) d,
+     refocus_out v c d -> ~dead_ckind k2.
 
   Proof with auto.
     intros k2 v k1 c d H H0.
@@ -36,52 +37,40 @@ Module RED_REF_SEM_Facts (R : RED_REF_SEM).
     - inversion H; dep_subst...
     - apply dec_context_from_dead with ec k2 v in H0.
       assert (G := dec_context_correct ec k2 v).
-      dependent destruction H; inversion_ccons x; dep_subst; (* WAR: unbound x *)
+      dependent destruction H; inversion_ccons x; dep_subst; (* WARRNING: unbound x *)
       match goal with H : dec_context ?ec ?k ?v = _ |- _ =>
       rewrite H in G
       end;
       solve [congruence].
   Qed.
 
-End RED_REF_SEM_Facts.
 
-
-
-
-(* Refocusing semantics is deterministic. *)
-
-Module RedRefSemDet (R : RED_REF_SEM) <: RED_SEM_DET R.
-
-  Module RF := RED_LANG_Facts R.
-  Import R RF.
-
-
-  Lemma dec_proc_is_pfunction :               forall t {k1 k2} (c : context k1 k2) d0 d1,
-      dec_proc t c d0 -> dec_proc t c d1 -> d0 = d1.
+  Lemma refocus_in_is_pfunction :             forall t {k1 k2} (c : context k1 k2) d0 d1,
+      refocus_in t c d0 -> refocus_in t c d1 -> d0 = d1.
 
   Proof.
     intros t k1 k2 c d0 d1 DE0 DE1. revert d1 DE1.
 
-    induction DE0 using dec_proc_Ind with 
-    (P  := fun _ t c d _ => forall d1, dec_proc t c d1    -> d = d1)
-    (P0 := fun _ v c d _ => forall d1, decctx_proc v c d1 -> d = d1);
+    induction DE0 using refocus_in_Ind with 
+    (P  := fun _ t c d _ => forall d1, refocus_in  t c d1    -> d = d1)
+    (P0 := fun _ v c d _ => forall d1, refocus_out v c d1 -> d = d1);
 
     intros;
 
     (* automated cases *)
     match goal with
 
-    | [ RD : (dec_proc ?t ?c ?d), DT1 : (dec_term ?t ?k = _) |- _ ] => 
+    | [ RD : (refocus_in ?t ?c ?d), DT1 : (dec_term ?t ?k = _) |- _ ] => 
              inversion RD; dep_subst; 
              match goal with DT2 : (dec_term ?t ?k = _) |- _ => 
                  rewrite DT2 in DT1; inversion DT1 end
 
-    | [ RC : (decctx_proc ?v (?ec=:?c) ?d), DC1 : (dec_context ?ec ?k ?v = _) |- _ ] => 
+    | [ RC : (refocus_out ?v (?ec=:?c) ?d), DC1 : (dec_context ?ec ?k ?v = _) |- _ ] => 
              dependent_destruction2 RC; inversion_ccons x2; dep_subst;
              match goal with DC2 : (dec_context ?ec' ?k' ?v' = _) |- _ => 
                  rewrite DC2 in DC1; inversion DC1 end
 
-    | [ RC : (decctx_proc ?v [.] ?d) |- _] => 
+    | [ RC : (refocus_out ?v [.] ?d) |- _] => 
              dependent_destruction2 RC
 
     end;
@@ -98,10 +87,10 @@ Module RedRefSemDet (R : RED_REF_SEM) <: RED_SEM_DET R.
     intros t k d0 d1 H H0.
     assert (~dead_ckind k) by apply H.
     rewrite <- (plug_empty t k) in H, H0.
-    apply dec_proc_eqv_dec in H...
-    apply dec_proc_eqv_dec in H0...
-    eauto 10 using dec_proc_is_pfunction.
+    apply refocus_in_eqv_dec in H...
+    apply refocus_in_eqv_dec in H0...
+    eauto 10 using refocus_in_is_pfunction.
   Qed.
 
 
-End RedRefSemDet.
+End RED_REF_SEM_Facts.
