refocusing_examples/miniml.v
@@ -423,15 +423,6 @@ Module MiniML_Strategy <: REF_STRATEGY MiniML_PreRefSem.
   Proof. REF_LANG_Help.prove_ec_wf. Qed.
 
 
-  (*Lemma search_order_antisym : forall k t ec ec0, 
-      k, t |~ ec << ec0 -> ~ k, t |~ ec0 << ec.
-  Proof.
-    intros k ? ec ec0.
-    destruct k, ec, ec0; 
-    solve [ autof ].
-  Qed.*)
-
-
   Lemma search_order_trans :  forall k t ec0 ec1 ec2, 
       k,t |~ ec0 << ec1 -> k,t |~ ec1 << ec2 -> 
       k,t |~ ec0 << ec2.
